src/Init/Data/Array/Lemmas.lean
@@ -3173,6 +3173,94 @@ theorem foldr_rel {l : Array α} {f g : α → β → β} {a b : β} (r : β →
   rcases l with ⟨l⟩
   simp
 
+-- /-! #### Further results about `back!` and `back?` -/
+
+-- theorem getLast_eq_iff_getLast_eq_some {xs : Array α} (h) : xs.back h = a ↔ xs.back? = some a := by
+--   sorry
+
+-- @[simp] theorem getLast?_eq_none_iff {xs : List α} : xs.getLast? = none ↔ xs = [] := by
+--   rw [getLast?_eq_head?_reverse, head?_eq_none_iff, reverse_eq_nil_iff]
+
+-- theorem getLast?_eq_some_iff {xs : List α} {a : α} : xs.getLast? = some a ↔ ∃ ys, xs = ys ++ [a] := by
+--   rw [getLast?_eq_head?_reverse, head?_eq_some_iff]
+--   simp only [reverse_eq_cons_iff]
+--   exact ⟨fun ⟨ys, h⟩ => ⟨ys.reverse, by simpa using h⟩, fun ⟨ys, h⟩ => ⟨ys.reverse, by simpa using h⟩⟩
+
+-- @[simp] theorem getLast?_isSome : l.getLast?.isSome ↔ l ≠ [] := by
+--   rw [getLast?_eq_head?_reverse, head?_isSome]
+--   simp
+
+-- theorem mem_of_getLast? {xs : List α} {a : α} (h : xs.getLast? = some a) : a ∈ xs := by
+--   obtain ⟨ys, rfl⟩ := getLast?_eq_some_iff.1 h
+--   exact mem_concat_self ys a
+
+-- @[deprecated mem_of_getLast? (since := "2024-10-21")] abbrev mem_of_getLast?_eq_some := @mem_of_getLast?
+
+-- @[simp] theorem getLast_reverse {l : List α} (h : l.reverse ≠ []) :
+--     l.reverse.getLast h = l.head (by simp_all) := by
+--   simp [getLast_eq_head_reverse]
+
+-- theorem head_eq_getLast_reverse {l : List α} (h : l ≠ []) :
+--     l.head h = l.reverse.getLast (by simp_all) := by
+--   rw [← getLast_reverse]
+
+-- @[simp] theorem getLast_append_of_ne_nil {l : List α} {h₁} (h₂ : l' ≠ []) :
+--     (l ++ l').getLast h₁ = l'.getLast h₂ := by
+--   simp only [getLast_eq_head_reverse, reverse_append]
+--   rw [head_append_of_ne_nil]
+
+-- theorem getLast_append {l : List α} (h : l ++ l' ≠ []) :
+--     (l ++ l').getLast h =
+--       if h' : l'.isEmpty then
+--         l.getLast (by simp_all [isEmpty_iff])
+--       else
+--         l'.getLast (by simp_all [isEmpty_iff]) := by
+--   split <;> rename_i h'
+--   · simp only [isEmpty_iff] at h'
+--     subst h'
+--     simp
+--   · simp [isEmpty_iff] at h'
+--     simp [h']
+
+-- theorem getLast_append_right {l : List α} (h : l' ≠ []) :
+--     (l ++ l').getLast (fun h => by simp_all) = l'.getLast h := by
+--   rw [getLast_append, dif_neg (by simp_all)]
+
+-- theorem getLast_append_left {l : List α} (w : l ++ l' ≠ []) (h : l' = []) :
+--     (l ++ l').getLast w = l.getLast (by simp_all) := by
+--   rw [getLast_append, dif_pos (by simp_all)]
+
+-- @[simp] theorem getLast?_append {l l' : List α} : (l ++ l').getLast? = l'.getLast?.or l.getLast? := by
+--   simp [← head?_reverse]
+
+-- theorem getLast_filter_of_pos {p : α → Bool} {l : List α} (w : l ≠ []) (h : p (getLast l w) = true) :
+--     getLast (filter p l) (ne_nil_of_mem (mem_filter.2 ⟨getLast_mem w, h⟩)) = getLast l w := by
+--   simp only [getLast_eq_head_reverse, ← filter_reverse]
+--   rw [head_filter_of_pos]
+--   simp_all
+
+-- theorem getLast_filterMap_of_eq_some {f : α → Option β} {l : List α} {w : l ≠ []} {b : β} (h : f (l.getLast w) = some b) :
+--     (filterMap f l).getLast (ne_nil_of_mem (mem_filterMap.2 ⟨_, getLast_mem w, h⟩)) = b := by
+--   simp only [getLast_eq_head_reverse, ← filterMap_reverse]
+--   rw [head_filterMap_of_eq_some (by simp_all)]
+--   simp_all
+
+-- theorem getLast?_flatMap {L : List α} {f : α → List β} :
+--     (L.flatMap f).getLast? = L.reverse.findSome? fun a => (f a).getLast? := by
+--   simp only [← head?_reverse, reverse_flatMap]
+--   rw [head?_flatMap]
+--   rfl
+
+-- theorem getLast?_flatten {L : List (List α)} :
+--     (flatten L).getLast? = L.reverse.findSome? fun l => l.getLast? := by
+--   simp [← flatMap_id, getLast?_flatMap]
+
+-- theorem getLast?_replicate (a : α) (n : Nat) : (replicate n a).getLast? = if n = 0 then none else some a := by
+--   simp only [← head?_reverse, reverse_replicate, head?_replicate]
+
+-- @[simp] theorem getLast_replicate (w : replicate n a ≠ []) : (replicate n a).getLast w = a := by
+--   simp [getLast_eq_head_reverse]
+
 /-! Content below this point has not yet been aligned with `List`. -/
 
 /-! ### sum -/
@@ -3226,7 +3314,9 @@ theorem getElem?_lt
 theorem getElem?_ge
     (a : Array α) {i : Nat} (h : i ≥ a.size) : a[i]? = none := dif_neg (Nat.not_lt_of_le h)
 
-@[simp] theorem get?_eq_getElem? (a : Array α) (i : Nat) : a.get? i = a[i]? := rfl
+set_option linter.deprecated false in
+@[deprecated "`get?` is deprecated" (since := "2025-02-12"), simp]
+theorem get?_eq_getElem? (a : Array α) (i : Nat) : a.get? i = a[i]? := rfl
 
 @[deprecated getElem?_eq_none (since := "2024-12-11")]
 theorem getElem?_len_le (a : Array α) {i : Nat} (h : a.size ≤ i) : a[i]? = none := by
@@ -3234,15 +3324,17 @@ theorem getElem?_len_le (a : Array α) {i : Nat} (h : a.size ≤ i) : a[i]? = no
 
 @[deprecated getD_getElem? (since := "2024-12-11")] abbrev getD_get? := @getD_getElem?
 
-@[simp] theorem getD_eq_get? (a : Array α) (i d) : a.getD i d = (a[i]?).getD d := by
-  simp only [getD, get_eq_getElem, get?_eq_getElem?]; split <;> simp [getD_getElem?, *]
+@[simp] theorem getD_eq_getD_getElem? (a : Array α) (i d) : a.getD i d = a[i]?.getD d := by
+  simp only [getD, get_eq_getElem]; split <;> simp [getD_getElem?, *]
+
+@[deprecated getD_eq_getD_getElem? (since := "2025-02-12")] abbrev getD_eq_get? := @getD_eq_getD_getElem?
 
 theorem get!_eq_getD [Inhabited α] (a : Array α) : a.get! n = a.getD n default := rfl
 
 theorem get!_eq_getElem? [Inhabited α] (a : Array α) (i : Nat) :
-    a.get! i = (a.get? i).getD default := by
+    a.get! i = a[i]?.getD default := by
   by_cases p : i < a.size <;>
-  simp only [get!_eq_getD, getD_eq_get?, getD_getElem?, p, get?_eq_getElem?]
+  simp only [get!_eq_getD, getD_eq_getD_getElem?, getD_getElem?, p]
 
 /-! # ofFn -/
 
@@ -3325,11 +3417,15 @@ theorem getElem?_size_le (a : Array α) (i : Nat) (h : a.size ≤ i) : a[i]? = n
 theorem getElem_mem_toList (a : Array α) (h : i < a.size) : a[i] ∈ a.toList := by
   simp only [← getElem_toList, List.getElem_mem]
 
+set_option linter.deprecated false in
+@[deprecated "`Array.get?` is deprecated, use `a[i]?` instead." (since := "2025-02-12")]
 theorem get?_eq_get?_toList (a : Array α) (i : Nat) : a.get? i = a.toList.get? i := by
   simp [← getElem?_toList]
 
-theorem get!_eq_get? [Inhabited α] (a : Array α) : a.get! n = (a.get? n).getD default := by
-  simp only [get!_eq_getElem?, get?_eq_getElem?]
+theorem get!_eq_getD_getElem? [Inhabited α] (a : Array α) : a.get! n = a[n]?.getD default := by
+  simp only [get!_eq_getElem?]
+
+@[deprecated get!_eq_getD_getElem? (since := "2025-02-12")] abbrev get!_eq_get? := @get!_eq_getD_getElem?
 
 theorem back!_eq_back? [Inhabited α] (a : Array α) : a.back! = a.back?.getD default := by
   simp [back!, back?, getElem!_def, Option.getD]; rfl
@@ -3939,8 +4035,6 @@ end Array
 
 namespace List
 
-@[deprecated back!_toArray (since := "2024-10-31")] abbrev back_toArray := @back!_toArray
-
 @[deprecated setIfInBounds_toArray (since := "2024-11-24")] abbrev setD_toArray := @setIfInBounds_toArray
 
 end List
@@ -3961,9 +4055,6 @@ abbrev getElem_fin_eq_toList_get := @getElem_fin_eq_getElem_toList
 
 @[deprecated "Use reverse direction of `getElem?_toList`" (since := "2024-10-17")]
 abbrev getElem?_eq_toList_getElem? := @getElem?_toList
-
-@[deprecated get?_eq_get?_toList (since := "2024-10-17")]
-abbrev get?_eq_toList_get? := @get?_eq_get?_toList
 
 @[deprecated getElem?_swap (since := "2024-10-17")] abbrev get?_swap := @getElem?_swap
 
