src/Init/Data/List/Basic.lean
@@ -246,46 +246,6 @@ theorem lex_cons_cons [BEq α] {a b} {as bs : List α} :
 
 /-! ## Alternative getters -/
 
-/-! ### get? -/
-
-/--
-Returns the `i`-th element in the list (zero-based).
-
-If the index is out of bounds (`i ≥ as.length`), this function returns `none`.
-Also see `get`, `getD` and `get!`.
--/
-def get? : (as : List α) → (i : Nat) → Option α
-  | a::_,  0   => some a
-  | _::as, n+1 => get? as n
-  | _,     _   => none
-
-@[simp] theorem get?_nil : @get? α [] n = none := rfl
-@[simp] theorem get?_cons_zero : @get? α (a::l) 0 = some a := rfl
-@[simp] theorem get?_cons_succ : @get? α (a::l) (n+1) = get? l n := rfl
-
-theorem ext_get? : ∀ {l₁ l₂ : List α}, (∀ n, l₁.get? n = l₂.get? n) → l₁ = l₂
-  | [], [], _ => rfl
-  | _ :: _, [], h => nomatch h 0
-  | [], _ :: _, h => nomatch h 0
-  | a :: l₁, a' :: l₂, h => by
-    have h0 : some a = some a' := h 0
-    injection h0 with aa; simp only [aa, ext_get? fun n => h (n+1)]
-
-/-! ### getD -/
-
-/--
-Returns the `i`-th element in the list (zero-based).
-
-If the index is out of bounds (`i ≥ as.length`), this function returns `fallback`.
-See also `get?` and `get!`.
--/
-def getD (as : List α) (i : Nat) (fallback : α) : α :=
-  (as.get? i).getD fallback
-
-@[simp] theorem getD_nil : getD [] n d = d := rfl
-@[simp] theorem getD_cons_zero : getD (x :: xs) 0 d = x := rfl
-@[simp] theorem getD_cons_succ : getD (x :: xs) (n + 1) d = getD xs n d := rfl
-
 /-! ### getLast -/
 
 /--
